Lean4Lean/Std/NodupKeys.lean
@@ -1,4 +1,5 @@
 import Std.Data.List.Perm
+import Std.Tactic.SeqFocus
 
 namespace List
 def NodupKeys (l : List (α × β)) : Prop := Nodup (l.map (·.1))
