Lean4Lean/Verify/UnionFind.lean
@@ -84,13 +84,13 @@ theorem root_link {self : UnionFind} {x y : Fin self.size}
         rw [← root_parent, go (m.parent i)]
         rw [hm i]; split <;> [subst i; rw [root_parent]]
         simp [root_eq_self.2 xroot, root_eq_self.2 yroot]
+    termination_by m.rankMax - m.rank i
     exact ⟨x, .inl rfl, go⟩
   if hr : self.rank y < self.rank x then
     exact this xroot yroot fun i => by simp [parent_link, h, hr]
   else
     simpa (config := {singlePass := true}) [or_comm] using
       this yroot xroot fun i => by simp [parent_link, h, hr]
-termination_by go => m.rankMax - m.rank i
 
 def Equiv (self : UnionFind) (a b : Nat) : Prop := self.root a = self.root b
 
